### E7.1

$\Delta s = 1 + \frac{Ks(s+4)}{s^2+2s+2} = 0$  
$1 + \frac{Ks(s+4)}{s^2+2s+2} = 1 + 
 \frac{z(s)}{p(s)}$  
>(1)  
$p(s)=0, s = -1 \pm j, \; n = 2$  
$z(s)=0, s = 0, 4, \; m = 2$  
(2)  
$n=m$, 점근선 X  
(3)  
$\theta_1+\theta_2+\theta_3+\theta_4=180+360k$  
$\theta_1=296.57$  
$\theta_2=0, \theta_3=180, \theta_4=63.43$  
(4) 
$s^2+2s+2+Ks(s+4)=0$  
$K=-\frac{s^2+2s+2}{s(s+4)}$  
$\frac{dK}{ds}=0$  
$s=-1.24$

(a)  
![Image](https://github.com/user-attachments/assets/7717e0c2-63ab-4202-90ba-6e9641df6ccb)  
![Image](https://github.com/user-attachments/assets/cc1499d4-838a-40e6-893a-d5a0c1221301)  

(b)  
$1 + \frac{Ks(s+4)}{s^2+2s+2} = 0$  
$s^2+2s+2 + Ks(s+4) = 0$  
$(K+1)s^2 + 2(2K+1)s + 2 = 0$  
$s = \frac{-(2K+1) \pm \sqrt{(2K+1)^2-2(K+1)}}{K+1}$  
$(2K+1)^2-2(K+1)=0$  
$K=0.31 or -0.81$  
$\therefore K=0.31$  

(c)  
$s=\frac{-(2K+1)}{K+1}, \; K=0.31$  
$\therefore s = -1.24$  

(d)  
$(K+1)s^2 + 2(2K+1)s + 2 = 0$  
$s^2+\frac{2(2K+1)}{K+1}s+\frac{2}{K+1} = s^2+2.47s+1.35 = 0$  
$s^2+2 \zeta \omega_n s+\omega_n^2 = 0$  
$\omega_n=1.24, \zeta=1.00$  
$\therefore T_s=\frac{4}{\zeta \omega_n} = 3.23$  

### E7.2  

$L(s)=\frac{K}{s(s+1)(s^2+10s+24)}=\frac{z(s)}{p(s)}$  
>(1)  
$p(s)=0, s = 0, -1, -4, -6 \; n = 4$  
$z(s)=0, \; m = 0$  
(2)  
$\sigma_A = \frac{\Sigma(poles)-\Sigma(zeros)}{n-m} = -2.75$  
$\phi_A = \frac{2k+1}{n-m} \cdot 180 = \frac{2k+1}{4} \cdot 180 = 45^\circ, 135^\circ, 225^\circ, 315^\circ$  
(3)  
$\theta_1+\theta_2+\theta_3+\theta_4=180+360k$  
$\theta_1=0$  
$\theta_2=180, \theta_3=0, \theta_4=1180$  
(4)  
$1+L(s)=1+\frac{K}{s(s+1)(s^2+10s+24)}= 0$  
$s(s+1)(s^2+10s+24)+K=0$  
$K=-s(s+1)(s^2+10s+24)$  
$\frac{dK}{ds}=0$  
$s=-0.44, -2.60, -5.21$  







(a)  
$G_c(s)=\frac{K}{0.2s+1}$  
$G(s)=\frac{100}{s^2+25s+100}$  
$\therefore S(s)=\frac{1}{1+G_c(s)G(s)}=\frac{(s+5)^2(s+20)}{(s^3+30s^2+225s+500K+500)}$


### E7.5
### E7.6   
### E7.21
### AP7.14
