#P2.7

$\frac{v_{1}(t)-0}{R}=C\frac{\text{d}(0-v_{2}(t))}{\text{d}t}+0$  
$\frac{v_{1}(t)}{R}=-C\frac{\text{d}v_{2}(t)}{\text{d}t}$  

라플라스 변환  
$\frac{V_{1}(s)}{R}=-Cs{V_{2}(s)}$  
$$\therefore\frac{V_{2}(s)}{V_{1}(s)}=-\frac{1}{RCs}$$


---
#P2.12

$Y(s)=R(s)\frac{K}{s+50}$  
$\mathcal{L}(r(t))=\mathcal{L}(u(t))=\frac{1}{s}$  
$Y(s)=\frac{K}{s(s+50)}=\frac{K}{50}(\frac{1}{s}-\frac{1}{s+50})$  
$y(t)=\mathcal{L^{-1}}(Y(s))=\frac{K}{50}(1-e^{-50t})$  
$\displaystyle\lim_{t\rarr\infin}{y(t)}=\frac{K}{50}=1$  
$$\therefore K=50$$


---
#P2.15

$mx''(t)+bx'(t)+kx(t)=\delta(t)$  

라플라스 변환  
$ms^2X(s)+bsX(s)+kX(s)=1$  
$X(s)(ms^2+bs+k)=1$  
$X(s)=\frac{1}{ms^2+bs+k}$  

매트랩으로 역변환  
$$\therefore x(t)=\frac{2m\sin(\frac{t\sqrt{-b^2+4km}}{2m})e^{\frac{-bt}{2m}}}{\sqrt{-b^2+4km}}$$


---
#P2.26

M에 관하여  
$F(t)+b\frac{\text{d}(y(t)-x(t))}{\text{d}t}+k(y(t)-x(t))=M\frac{\text{d}^2x}{\text{d}^2t}$

라플라스 변환  
$F(s)+bs(Y(s)-X(s))+k(Y(s)-X(s))=Ms^2X(s)$  
$F(s)=X(s)(Ms^2+bs+k)-Y(s)(bs+k)\cdots(1)$  

m에 관하여  
$-b\frac{\text{d}(y(t)-x(t))}{\text{d}t}-k(y(t)-x(t))=m\frac{\text{d}^2y}{\text{d}^2t}$  

라플라스 변환  
$ms^2Y(s)+bs(Y(s)-X(s))+k(Y(s)-X(s))=0$  
$X(s)=\frac{Y(s)(ms^2+bs+k)}{bs+k}\cdots(2)$  

(1)에 (2)대입  
$F(s)=Y(s)\frac{(ms^2+bs+k)}{bs+k}(Ms^2+bs+k)-Y(s)(bs+k)$  
$$\therefore\frac{Y(s)}{F(s)}=\frac{bs+k}{mMs^4+s^2(m+M)(bs+k)}$$

---
#P2.37

(a)  
$-K_{1}x(t)+K_{2}(y(t)-x(t))=m_{1}\frac{\text{d}^2x(t)}{\text{d}t^2}$  
$-K_{2}(y(t)-x(t))-u(t)=m_{2}\frac{\text{d}^2y(t)}{\text{d}t^2}$  

(b)  
$m_{1}=m_{2}=1, K_{1}=K_{2}=1$ 대입  
$m\frac{\text{d}^2x(t)}{\text{d}t^2}+2x(t)=y(t)$  
$-\frac{\text{d}^2y(t)}{\text{d}t^2}-y(t)+x(t)=u(t)$  

라플라스 변환  
$s^2X(s)+2X(s)=Y(s)$  
$X(s)=\frac{Y(s)}{s^2+2}\cdots(1)$  
$-s^2Y(s)-Y(s)+X(s)=U(s)\cdots(2)$  

(2)에 (1)대입  
$-s^2Y(s)-Y(s)+\frac{Y(s)}{s^2+2}=U(s)$  
$$\therefore\frac{Y(s)}{U(s)}=-\frac{s^2+2}{s^4+3s^2+1}$$

