### P3.1  

(a)  
$\therefore y(t)=x_1(t),  \frac{dy(t)}{dt}=x_2(t)$  

(b)  
$F(t)-ky(t)-b\frac{y(t)}{dt}=M\frac{dy(t)}{dt^2}$  

$\therefore \frac{d{x_2}(t)}{dt}=-\frac{k}{M}x_1(t)-\frac{b}{M}x_2(t)+\frac{1}{M}F(t)$  
&nbsp; &nbsp; $\frac{{dx_1}(t)}{dt}=x_2(t)$  

(c)  

$$\therefore \dot{x}(t)=
\begin{bmatrix} 0 & 1 \\ -\frac{k}{M} & -\frac{b}{M} \end{bmatrix}
x(t)+\begin{bmatrix} 0 \\ \frac{1}{M} \end{bmatrix}
F(t)$$  
$$y(t)=\begin{bmatrix} 1 & 0 \end{bmatrix}\mathbf{x}_1(t)$$  

---
### P3.3  

KVL 적용  
$-v_1(t)+L\frac{di_L(t)}{dt}-v_c(t)+v_2(t)=0$  
$-v_1(t)+L\frac{dx_1(t)}{dt}-x_2(t)+v_2(t)=0$  

$\frac{dx_1(t)}{dt}=\frac{1}{L}x_2(t)+\frac{1}{L}v_1(t)-\frac{1}{L}v_2(t)$  

KCL 적용   
$i_L(t)+\frac{V_0}{R}=i_{c}(t), V_0=v_2(t)-v_c(t)=v_2(t)-x_2(t)$  
$i_L(t)=x_1(t), i_c(t)=-C\frac{dv_c(t)}{dt}=-C\frac{dx_2(t)}{dt}$  
$x_1(t)+\frac{v_2(t)-x_2(t)}{R}=-C\frac{dx_2(t)}{dt}$  

$\frac{dx_2(t)}{dt}=-\frac{1}{C}x_1(t)+\frac{1}{RC}x_2(t)-\frac{1}{RC}v_2(t)$  

$$\therefore \dot{\mathbf{x}}(t)=\begin{bmatrix} 0&\frac{1}{L} \\ -\frac{1}{C}&\frac{1}{RC} \end{bmatrix}\mathbf{x}(t)+\begin{bmatrix}\frac{1}{L} & -\frac{1}{L} \\ 0&-\frac{1}{RC} \end{bmatrix}\mathbf{v}(t)$$  

---
### P3.5  

a)  
$(R(s)-Y(s))\frac{s+2}{s(s-3)(s+8)}=Y(s)$  
$$\therefore T(s)=\frac{Y(s)}{R(s)}=\frac{s+2}{s^3+5s^2-23s+2}$$  

b)  
$\frac{Y(s)}{R(s)}=\frac{s+2}{s^3+5s^2-23s+2}\frac{Z(s)}{Z(s)}$ 

$Y(s)=(s+2)Z(s)$  
$R(s)=(s^3+5s^2-23s+2)Z(s)$    

$y(t)=\frac{dz(t)}{dt}+2z(t)$  
$r(t)=\frac{d^3z(t)}{dt^3}+5\frac{d^2z(t)}{dt^2}-23\frac{dz(t)}{dt}+2z(t)$  

$x_1(t)=z(t)$  
$x_2(t)=\frac{dx_1(t)}{dt}=\frac{dz(t)}{dt}$  
$x_3(t)=\frac{dx_2(t)}{dt}=\frac{d^2z(t)}{dt^2}$  

$\frac{dx_1(t)}{dt}=x_2(t)$  
$\frac{dx_2(t)}{dt}=x_3(t)$  
$\frac{dx_3(t)}{dt}=-2x_1(t)+23x_2(t)-5x_3(t)+r(t)$  

$$\therefore \dot{\mathbf{x}}(t)=\begin{bmatrix} 
0&1&0 \\
0&0&1 \\
-2&23&-5
\end{bmatrix}\mathbf{x}(t)+\begin{bmatrix}
0 \\ 0 \\ 1
\end{bmatrix}r(t)$$  
$$y(t)=\begin{bmatrix} 2&1&0 \end{bmatrix}\mathbf{x}(t)$$

---
### P3.12  

(a)
$T(s)=\frac{Y(s)}{R(s)}=\frac{8s+40}{s^3+12s^2+44s+48}\frac{Z(s)}{Z(s)}$  

$Y(s)=(8s+40)Z(s)$  
$R(s)=(s^3+12s^2+44s+48)Z(s)$    

$y(t)=8\frac{dz(t)}{dt}+40z(t)$  
$r(t)=\frac{d^3z(t)}{dt^3}+12\frac{d^2z(t)}{dt^2}+44\frac{dz(t)}{dt}+48z(t)$  

$x_1(t)=z(t)$  
$x_2(t)=\frac{dx_1(t)}{dt}=\frac{dz(t)}{dt}$  
$x_3(t)=\frac{dx_2(t)}{dt}=\frac{d^2z(t)}{dt^2}$  

$\frac{dx_1(t)}{dt}=x_2(t)$  
$\frac{dx_2(t)}{dt}=x_3(t)$  
$\frac{dx_3(t)}{dt}=-48x_1(t)-44x_2(t)-12x_3(t)+r(t)$  

$$\therefore \dot{\mathbf{x}}(t)=\begin{bmatrix} 
0&1&0 \\
0&0&1 \\
-48&-44&-12
\end{bmatrix}\mathbf{x}(t)+\begin{bmatrix}
0 \\ 0 \\ 1
\end{bmatrix}r(t)$$  
$$y(t)=\begin{bmatrix} 40&8&0 \end{bmatrix}\mathbf{x}(t)$$

b)  

$[sI-A] =
\begin{bmatrix}
 s & -1 & 0 \\
 0 & s & -1 \\
 48 & 44 & s+12
\end{bmatrix}$  

$\Phi(s)=[s\mathbf{I}-\mathbf{A}]^{-1}=\frac{1}{s^3 + 12s^2 + 44s + 48}
\begin{bmatrix}
s^2 + 12s + 44&s + 12&1 \\
-48 & s(s + 12) & s \\
-48s & -4(11s + 12) & s^2
\end{bmatrix}$  

$$\therefore \Phi(t)=\mathcal{L}^{-1}(\Phi(s))=\begin{bmatrix}
3e^{-2t}-3e^{-4t}+e^{-6t} & \frac{5e^{-2t}}{4}-2e^{-4t}+\frac{3e^{-6t}}{4} & \frac{e^{-2t}}{8}-\frac{e^{-4t}}{4}+\frac{e^{-6t}}{8} \\
12e^{-4t}-6e^{-2t}-6e^{-6t} & 8e^{-4t}-\frac{5e^{-2t}}{2}-\frac{9e^{-6t}}{2} & e^{-4t}-\frac{e^{-2t}}{4}-\frac{3e^{-6*t}}{4} \\
12e^{-2t}-48e^{-4t}+36e^{-6t} & 5e^{-2t}-32e^{-4t}+27e^{-6t} & \frac{e^{-2t}}{2}-4e^{-4t}+\frac{9e^{-6t}}{2}
\end{bmatrix}
$$  

---
### P3.17  

$A=\begin{bmatrix}
1 & 1 & -1 \\ 4 & 3 & 0 \\ -2 & 1 & 10
\end{bmatrix}$  
$B=\begin{bmatrix} 0 \\ 0 \\ 4 \end{bmatrix}$  
$C=\begin{bmatrix} 1 & 0 & 0 \end{bmatrix}$  
$D=0$  

$X(s)=[s\mathbf{I}-\mathbf{A}]^{-1}BU(s)$  
$Y(s)=CX(s)+DU(s)$  
$Y(s)=[C[s\mathbf{I}-\mathbf{A}]^{-1}B+D]U(s)$  

$G(s)=\frac{Y(s)}{U(s)}=C[s\mathbf{I}-\mathbf{A}]^{-1}B=\frac{-4(s-3)}{s^3-14s^2+37s+20}$  

$$\therefore G(s)=\frac{Y(s)}{U(s)}=\frac{-4(s-3)}{s^3-14s^2+37s+20}$$




