### P4.8
(a)  
$G_c(s)=\frac{K}{0.2s+1}$  
$G(s)=\frac{100}{s^2+25s+100}$  
$\therefore S(s)=\frac{1}{1+G_c(s)G(s)}=\frac{(s+5)^2(s+20)}{(s^3+30s^2+225s+500K+500)}$

(b)  
$Y(s)=G_c(s)G(s)S(s)R(s)+G(s)S(s)T_d(s)$  
if $R(s)=0, \ Y(s)=G(s)S(s)T_d(s)$  
$\therefore T_d(s)=\frac{Y(s)}{G(s)S(s)}=\frac{s^3+30s^2+255s+500K+500}{100(s+5)}Y(s)$

(c)  
$|Y(s)|<0.1|T_d(s)|$  
$|G(s)S(s)|=|\frac{100s+500}{s^3+30s^2+255s+500K+500}|<0.1$  
if s = 0, $|G(s)S(s)|=\frac{1}{K+1}<0.1$  
$\therefore K>9$

### P4.12
(a)  
$T(s)=\frac{G(s)}{1+G(s)H(s)}$  
$G(s)=\frac{K_1}{s+4}\frac{K_2}{s-1}, \ H(s)=6$  
$\therefore T_1(s)=\frac{K_1K_2}{s^2+3s+6K_1K_2-4}$

$G_a(s)=\frac{K_1}{s+4}, \ H_a(s)=-2$  
$G_b(s)=\frac{K_2}{s-1}, \ H_b(s)=2$  
$\therefore T_2(s)=\frac{G_a(s)}{1+G_a(s)H_a(s)}\frac{G_b(s)}{1+G_b(s)H_b(s)}=\frac{K_1K_2(2K_2+s-1)}{(s-1)^2(s-2K_1+4)}$

(b)  
$S(s)=1-T(s)$  
$\therefore \ S_1(s)=1-T_1(s)=\frac{s^2 +3\,s+5\,K_1 \,K_2 -4}{s^2 +3\,s+6\,K_1 \,K_2 -4}$  
$S_2(s)=1-T_2(s)=1-\frac{K_1 \,K_2 \,{\left(2\,K_2 +s-1\right)}}{{{\left(s-1\right)}}^2 \,{\left(s-2\,K_1 +4\right)}}$  

### P4.17
(a)  
$G_1(s)=\frac{KK_m}{R_f}=K, \ G_2(s)=\frac{1}{s(Js+b)}=\frac{1}{s(0.1s+1)}$  
$G(s)=G_1(s)G_2(s)=\frac{K}{s(Js+b)}$  
$H(s)=K_f=1$  
$T(s)=\frac{G(s)}{1+G(s)H(s)}=\frac{K(s+10)}{10K+1s+Ks}$  
$\theta(s)=T(s)\theta_d(s)=\frac{G(s)}{1+G(s)H(s)}=\frac{K(s+10)}{10K+1s+Ks}\frac{1}{s}$  
$K=20$  
$\therefore \theta(s)=\frac{2s+20}{s(3s+20)}$  

(b)  
$S(s)=1-T(s)$  
$\theta(s)=G(s)S(s)\theta_d(s)+G(s)S(s)T_d(s)$  
$\theta_d(s)=0, \ T_d(s)=\frac{A}{s}$  
$\therefore \theta(s)=\frac{A\,K\,{\left(s+10\right)}}{s\,{\left(10\,K+10\,s+K\,s\right)}}$  

(c)  
$E(s)=S(s)R(s)-S(s)G(s)T_d(s)$  
$r(t)=t, \ R(s)=\frac{1}{s^2}, \ T_d(s)=0$  
$ess=\lim_{t \to \infty} e(t)=\lim_{s \to 0} sE(s)$  
$\therefore ess=\lim_{s \to 0} \frac{S(s)}{s}=\frac{1}{K}$

### P5.3
$G(s)=\frac{K}{s(s+K_1)}$  
$T(s)=\frac{G(s)}{1+G(s)}=\frac{K}{s^2 +K_1 \,s+K}$  
$S(s)=1-T(s)=\frac{s\,{\left(K_1 +s\right)}}{s^2 +K_1 \,s+K}$  
$E(s)=S(s)R(s)$  
$r(t)=t, \ R(s)=\frac{1}{s^2}$  
$ess=\lim_{t \to \infty} e(t)=\lim_{s \to 0} sE(s)$  
$ess=\lim_{s \to 0} \frac{S(s)}{s}=\frac{K_1}{K}=5$  
$\therefore K_1=5K$

### P5.5
(a)  
$\tau_1=1, \ \tau_2=0$  
$P.O. =100e^{-\frac{\zeta\pi}{\sqrt{1-\zeta^2}}}\leqq5\%, \ \zeta=0.7$  
$G(s)=\frac{K_2(\tau_1s+1)K_1}{(\tau_2s+1)s^2}=\frac{K_1K_2(s+1)}{s^2}$  
$T(s)=\frac{G(s)}{1+G(s)}=\frac{K_1 \,K_2 \,{\left(s+1\right)}}{s^2+K_1K_2(s+1)}$  
$Y(s)=T(s)R(s)=\frac{\omega_n^2}{s^2+2\zeta\omega_ns+\omega_n^2}R(s)$  
$2\zeta\omega_n=K_1K_2=K, \ \omega_n^2=K_1K_2=K$  
$\omega_n=1.4$  
$\therefore K=1.96$

(b)  
$r(t)=1$  
$\therefore ess=\frac{1}{1+K}=0.3378$  

$r(t)=s$  
$\therefore ess=\frac{1}{K}=0.5102$  

### P5.7
(a)  
$r(t)=t$  
$ess=\frac{1}{K_3}=0.01$  
$K_3=100$  

(b)  
$I=25$  
$G_1(s)=\frac{K_1K_2}{Is}, H(s)=K_3$  
$T_1(s)=\frac{G_1(s)}{1+G_1(s)H(s)}$  
$G_2(s)=T_1(s)\frac{1}{s}$  
$T_2(s)=\frac{G_2(s)}{1+G_2(s)}=\frac{\frac{K_1 \,K_2}{I} }{s^2 +\frac{K_1 \,K_2 \,K_3}{I} \,s+\frac{K_1 \,K_2}{I} }$  
$2\zeta\omega_n=\frac{K_1K_2K_3}{I}, \ \omega_n^2=\frac{K_1K_2}{I}$  
$P.O.=100e^{-\frac{\zeta\pi}{\sqrt{1-\zeta^2}}}\leqq10\%, \ \zeta=0.6$  
$1.2\omega_n=\frac{K_1K_2K_3}{25}, \ \omega_n^2=\frac{K_1K_2}{25}$  
$1.2\omega_n=\omega_n^2K_3, \ \omega_n=\frac{1.2}{K_3}$
$\therefore K_1K_2=25\omega_n^2=\frac{36}{{K_3}^2}$  

### P5.10
(a)  
(https://github.com/GitCatcatcat/homework/issues/4#issue-2736609874)

(b) 
$R_a=L_a=J=b=K_m=K_b=1$  
$T(s)=\frac{K_m}{(R_a+L_as)(Js+b)+K_bK_m}=\frac{1}{(s+1)^2+1}$  
$S(s)=1-T(s), \ R(s)=\frac{1}{s}$  
$ess=\lim_{s \to 0} sE(s)=\lim_{s \to 0} sS(s)R(s)$  
$\therefore ess = \frac{1}{2}$  


(c)  
$R_a=L_a=J=b=1$  
$T(s)=\frac{K_m}{(R_a+L_as)(Js+b)+K_bK_m}=\frac{K_m}{s^2+2s+1+K_bK_m}$  
$Y(s)=T(s)R(s)=\frac{\omega_n^2}{s^2+2\zeta\omega_ns+\omega_n^2}R(s)$  
$R(s)=\frac{1}{s}$  
$P.O.=15\%, \ \zeta=0.516$  
$2\zeta\omega_n=2, \ \omega_n=\frac{1}{\zeta}=1.938$  
${\omega_n}^2=K_m=1+K_bK_m=3.7558$  
$\therefore K_b=\frac{K_m-1}{K_m}=0.7337$  

### P6.1
매트랩에서 실행
```
a=[1 5 2]  
b=[1 4 8 4]  
c=[1 2 -6 20]  
d=[1 1 2 12 10]  
e=[1 1 1 1 K]  
f=[1 1 2 0 1 6]  
g=[1 1 2 1 1 K]  

routh_hurwitz(a)  
routh_hurwitz(b)  
routh_hurwitz(c)  
routh_hurwitz(d)  
routh_hurwitz(e)  
routh_hurwitz(f)  
routh_hurwitz(g)  
```  

(a)  
$\begin{bmatrix}  
1.0 & 2.0 \\  
5.0 & 0 \\  
2.0 & 0  
\end{bmatrix}$  
stable  
number of roots in the right hand plane: 0

(b)
$\begin{bmatrix}  
1.0 & 8.0\\  
4.0 & 4.0\\  
7.0 & 0\\  
4.0 & 0  
\end{bmatrix}$  
stable  
number of roots in the right hand plane: 0

(c)
$\begin{bmatrix}  
1.0 & -6.0\\  
2.0 & 20.0\\  
-16.0 & 0\\  
20.0 & 0  
\end{bmatrix}$  
unstable  
number of roots in the right hand plane: 2

(d)
$\begin{bmatrix}  
1.0 & 2.0 & 10.0\\  
1.0 & 12.0 & 0\\  
-10.0 & 10.0 & 0\\  
13.0 & 0 & 0\\  
10.0 & 0 & 0  
\end{bmatrix}$  
unstable  
number of roots in the right hand plane: 2

(e)
$\begin{bmatrix}  
1.0 & 1.0 & K\\  
1.0 & 1.0 & 0\\  
\varepsilon  & K & 0\\  
-\frac{1.0\,{\left(K-1.0\,\varepsilon \right)}}{\varepsilon } & 0 & 0\\  
K & 0 & 0  
\end{bmatrix}$  
if $K=0$ stable

(f)
$\begin{bmatrix}  
1.0 & 2.0 & 1.0\\  
1.0 & 0 & 6.0\\  
2.0 & -5.0 & 0\\  
2.5 & 6.0 & 0\\  
-9.8 & 0 & 0\\  
6.0 & 0 & 0  
\end{bmatrix}$  
unstable  
number of roots in the right hand plane: 2

(g)
$\begin{bmatrix}  
1.0 & 2.0 & 1.0\\  
1.0 & 1.0 & K\\  
1.0 & 1.0-1.0\,K & 0\\  
K & K & 0\\  
-1.0\,K & 0 & 0\\  
K & 0 & 0  
\end{bmatrix}$  
if $K=0$ stable

### P6.6
(a)  
$CE=1+G_c(s)G(s)=0$  
$s^3 +8s^2 +40s+30=0$  
$\begin{bmatrix}  
1.0 & 40.0\\  
8.0 & 30.0\\  
36.25 & 0\\  
30.0 & 0  
\end{bmatrix}$  
stable

(b)  
$s^4 +2s^3 +5s^2+2s+10=0$  
$\begin{bmatrix}  
1.0 & 5.0 & 10.0\\  
1.0 & 1.0 & 0\\  
4.0 & 10.0 & 0\\  
-1.5 & 0 & 0\\  
10.0 & 0 & 0  
\end{bmatrix}$  
unstable

(c)  
$s^3 +4s^2 +3s+3=0$  
$\begin{bmatrix}  
1.0 & 1.0\\\
4.0 & 3.0\\\
0.25 & 0\\\
3.0 & 0  
\end{bmatrix}$  
stable

$$\therefore
\begin{bmatrix} 0 & 1 \\\ -\frac{k}{M} & -\frac{b}{M}
\end{bmatrix}$$